Don't pass a wf proof into InterpToPHOAS
Use a fail-value instead.  This makes it easier to compose with other
transformations.

src/Reflection/Named/InterpretToPHOAS.v
@@ -1,5 +1,6 @@
 Require Import Crypto.Reflection.Named.Syntax.
 Require Import Crypto.Reflection.Named.Wf.
+Require Import Crypto.Reflection.SmartMap.
 Require Import Crypto.Reflection.Syntax.
 Require Import Crypto.Util.PointedProp.
 
@@ -12,54 +13,52 @@ Module Export Named.
             {Name : Type}.
     Section with_var.
       Context {var : base_type_code -> Type}
-              {Context : Context Name var}.
+              {Context : Context Name var}
+              (failb : forall t, @Syntax.exprf base_type_code op var (Tbase t)).
+
+      Local Notation failf t (* : @Syntax.exprf base_type_code op var t*)
+        := (SmartPairf (SmartValf _ failb t)).
 
       Fixpoint interpf_to_phoas
                (ctx : Context)
                {t} (e : @Named.exprf base_type_code op Name t)
                {struct e}
-        : prop_of_option (wff ctx e) -> @Syntax.exprf base_type_code op var t
-        := match e in Named.exprf _ _ _ t return prop_of_option (wff ctx e) -> @Syntax.exprf base_type_code op var t with
+        : @Syntax.exprf base_type_code op var t
+        := match e in Named.exprf _ _ _ t return @Syntax.exprf base_type_code op var t with
            | Named.Var t' x
-             => match lookupb ctx x t' as v return prop_of_option (if v return bool then true else false) -> _ with
-                | Some v => fun _ => Var v
-                | None => fun b => match b : False with end
+             => match lookupb ctx x t' with
+                | Some v => Var v
+                | None => failf _
                 end
-           | Named.TT => fun _ => TT
+           | Named.TT => TT
            | Named.Pair tx ex ty ey
-             => fun Hwf : prop_of_option (Named.wff _ _ /\ Named.wff _ _)%option_pointed_prop
-                => let (Hwf'1, Hwf'2) := eta_and (proj1 (prop_of_option_and _ _) Hwf) in
-                   Pair (@interpf_to_phoas ctx tx ex Hwf'1) (@interpf_to_phoas ctx ty ey Hwf'2)
+             => Pair (@interpf_to_phoas ctx tx ex) (@interpf_to_phoas ctx ty ey)
            | Named.Op _ _ opc args
-             => fun Hwf
-                => Op opc (@interpf_to_phoas ctx _ args Hwf)
+             => Op opc (@interpf_to_phoas ctx _ args)
            | Named.LetIn _ n ex _ eC
-             => fun Hwf : prop_of_option (Named.wff _ _ /\ inject (forall k, prop_of_option (Named.wff _ _)))%option_pointed_prop
-                => let (Hwf'1, Hwf'2) := eta_and (proj1 (prop_of_option_and _ _) Hwf) in
-                   LetIn (@interpf_to_phoas ctx _ ex Hwf'1)
-                         (fun v
-                          => @interpf_to_phoas (extend ctx n v) _ eC (Hwf'2 _))
+             => LetIn (@interpf_to_phoas ctx _ ex)
+                      (fun v
+                       => @interpf_to_phoas (extend ctx n v) _ eC)
            end.
 
       Definition interp_to_phoas
                  (ctx : Context)
                  {t} (e : @Named.expr base_type_code op Name t)
-                 (Hwf : wf ctx e)
         : @Syntax.expr base_type_code op var (domain t -> codomain t)
-        := Abs (fun v => interpf_to_phoas (extend ctx (Abs_name e) v) (invert_Abs e) (Hwf v)).
+        := Abs (fun v => interpf_to_phoas (extend ctx (Abs_name e) v) (invert_Abs e)).
     End with_var.
 
     Section all.
-      Context {Context : forall var, @Context base_type_code Name var}.
+      Context {Context : forall var, @Context base_type_code Name var}
+              (failb : forall var t, @Syntax.exprf base_type_code op var (Tbase t)).
       Definition InterpToPHOAS_gen
                  (ctx : forall var, Context var)
                  {t} (e : @Named.expr base_type_code op Name t)
-                 (Hwf : forall var, wf (ctx var) e)
         : @Syntax.Expr base_type_code op (domain t -> codomain t)
-        := fun var => interp_to_phoas (ctx var) e (Hwf var).
+        := fun var => interp_to_phoas (failb var) (ctx var) e.
 
-      Definition InterpToPHOAS {t} e (Hwf : forall var, wf empty e)
-        := @InterpToPHOAS_gen (fun var => empty) t e Hwf.
+      Definition InterpToPHOAS {t} e
+        := @InterpToPHOAS_gen (fun var => empty) t e.
     End all.
   End language.
 End Named.
