src/Reflection/Named/InterpretToPHOASInterp.v
@@ -9,6 +9,7 @@ Require Import Crypto.Util.PointedProp.
 Require Import Crypto.Util.Decidable.
 Require Import Crypto.Util.Option.
 Require Import Crypto.Util.Tactics.BreakMatch.
+Require Import Crypto.Util.Tactics.DestructHead.
 
 Section language.
   Context {base_type_code : Type}
@@ -20,28 +21,33 @@ Section language.
           {interp_op : forall src dst, op src dst -> interp_flat_type interp_base_type src -> interp_flat_type interp_base_type dst}.
   Section with_context.
     Context {Context : Context Name interp_base_type}
-            {ContextOk : ContextOk Context}.
+            {ContextOk : ContextOk Context}
+            (failb : forall t, @Syntax.exprf base_type_code op interp_base_type (Tbase t)).
 
     Lemma interpf_interpf_to_phoas
           (ctx : Context)
           {t} (e : @Named.exprf base_type_code op Name t)
           (Hwf : prop_of_option (Named.wff ctx e))
       : Named.interpf (interp_op:=interp_op) (ctx:=ctx) e
-        = Some (Syntax.interpf interp_op (interpf_to_phoas ctx e Hwf)).
+        = Some (Syntax.interpf interp_op (interpf_to_phoas failb ctx e)).
     Proof.
       revert dependent ctx; induction e;
         repeat first [ progress intros
                      | progress subst
                      | progress inversion_option
+                     | progress destruct_head' and
                      | progress break_innermost_match_step
                      | progress unfold option_map, LetIn.Let_In in *
                      | apply (f_equal (@Some _))
                      | apply (f_equal (@interp_op _ _ _))
                      | progress simpl in *
-                     | solve [ eauto | congruence ]
+                     | progress autorewrite with push_prop_of_option in *
+                     | solve [ eauto | congruence | tauto ]
                      | match goal with
                        | [ H : forall ctx Hwf', Named.interpf ?e = Some _, Hwf : prop_of_option (Named.wff _ ?e) |- _ ]
                          => specialize (H _ Hwf)
+                       | [ H : forall ctx Hwf, Named.interpf ?e = Some _ |- Named.interpf ?e = Some _ ]
+                         => rewrite H by auto
                        end ].
     Qed.
 
@@ -51,15 +57,16 @@ Section language.
           (Hwf : Named.wf ctx e)
           v
       : Named.interp (interp_op:=interp_op) (ctx:=ctx) e v
-        = Some (Syntax.interp interp_op (interp_to_phoas ctx e Hwf) v).
+        = Some (Syntax.interp interp_op (interp_to_phoas failb ctx e) v).
     Proof.
-      unfold interp, interp_to_phoas, Named.interp; apply interpf_interpf_to_phoas.
+      unfold interp, interp_to_phoas, Named.interp; apply interpf_interpf_to_phoas; auto.
     Qed.
   End with_context.
 
   Section all.
     Context {Context : forall var, @Context base_type_code Name var}
-            {ContextOk : forall var, ContextOk (Context var)}.
+            {ContextOk : forall var, ContextOk (Context var)}
+            (failb : forall var t, @Syntax.exprf base_type_code op var (Tbase t)).
 
     Lemma Interp_InterpToPHOAS_gen
           {ctx : forall var, Context var}
@@ -67,15 +74,15 @@ Section language.
           (Hwf : forall var, Named.wf (ctx var) e)
           v
       : Named.interp (interp_op:=interp_op) (ctx:=ctx _) e v
-        = Some (Interp interp_op (InterpToPHOAS_gen ctx e Hwf) v).
-    Proof. apply interp_interp_to_phoas. Qed.
+        = Some (Interp interp_op (InterpToPHOAS_gen failb ctx e) v).
+    Proof. apply interp_interp_to_phoas; auto. Qed.
 
     Lemma Interp_InterpToPHOAS
           {t} (e : @Named.expr base_type_code op Name t)
           (Hwf : Named.Wf Context e)
           v
       : Named.interp (Context:=Context _) (interp_op:=interp_op) (ctx:=empty) e v
-        = Some (Interp interp_op (InterpToPHOAS e Hwf) v).
-    Proof. apply interp_interp_to_phoas. Qed.
+        = Some (Interp interp_op (InterpToPHOAS (Context:=Context) failb e) v).
+    Proof. apply interp_interp_to_phoas; auto. Qed.
   End all.
 End language.
